Getting rid of n0 and ns, gas parameters of loop1_decider0 that were not used because of overshadowing

CoqBB5/Deciders/Decider_Loop.v
@@ -7,8 +7,83 @@ From CoqBB5 Require Import BB52Statement.
 From CoqBB5 Require Import CustomTactics.
 From CoqBB5 Require Import TNF.
 From CoqBB5 Require Import ListTape.
+From CoqBB5 Require Import Prelims.
+From CoqBB5 Require Import Encodings.
 
-Fixpoint loop1_decider0(tm:TM Σ)(n:nat)(es:ListES)(d:Z)(ls:list (ListES*Z))(n0:nat)(ns:list nat):HaltDecideResult :=
+(* Begin: Loop decider implementation *)
+
+Fixpoint verify_loop1(h0 h1:ListES*Z)(ls0 ls1:list (ListES*Z))(n:nat)(dpos:Z):bool :=
+  let (es0,d0):=h0 in
+  let (es1,d1):=h1 in
+  St_eqb es0.(s) es1.(s) &&&
+  Σ_eqb es0.(m) es1.(m) &&&
+  (
+    match n with
+    | O =>
+      match dpos with
+      | Z0 => Z.eqb d1 d0
+      | Zpos _ =>
+        match es1.(r) with
+        | nil => Z.ltb d1 d0
+        | _ => false
+        end
+      | Zneg _ =>
+        match es1.(l) with
+        | nil => Z.ltb d0 d1
+        | _ => false
+        end
+      end
+    | _ => false
+    end |||
+    match ls0,ls1 with
+    | h0'::ls0',h1'::ls1' =>
+      verify_loop1 h0' h1' ls0' ls1' (Nat.pred n) dpos
+    | _,_ => false
+    end
+  ).
+
+Fixpoint find_loop1(h0 h1 h2:ListES*Z)(ls0 ls1 ls2:list (ListES*Z))(n:nat){struct ls1}:bool :=
+  (
+    (let (es0,d0):=h0 in
+    let (es1,d1):=h1 in
+    St_eqb es0.(s) es1.(s) &&&
+    let (es2,d2):=h2 in
+    St_eqb es0.(s) es2.(s) &&&
+
+    Σ_eqb es0.(m) es1.(m) &&&
+    Σ_eqb es0.(m) es2.(m) &&&
+
+    (verify_loop1 h0 h1 ls0 ls1 (S n) (d0-d1)))
+  ) |||
+
+  match ls2,ls1 with
+  | h3::h2'::ls2',h1'::ls1' =>
+    find_loop1 h0 h1' h2' ls0 ls1' ls2' (S n)
+  | _,_ => false
+  end.
+
+Definition find_loop1_0(h0 h1:ListES*Z)(ls:list (ListES*Z)):bool :=
+match ls with
+| h2::ls' => find_loop1 h0 h1 h2 (h1::ls) ls ls' O
+| nil => false
+end.
+
+(** Loop decider aux function
+
+Args:
+  - tm: TM Σ, the Turing machine that the NGramCPS decider is checking.
+  - n: nat, gas parameter
+  - es:ListES, current configuration (ExecState), using the `ListES` representation, see ListTape.v
+  - d: Z, current head position index on the tape
+  - ls: list (ListES*Z), list of visited configurations and head positions
+
+Returns:
+  - HaltDecideResult:
+    - Result_Halt s i: the Turing machine halts at configuration (s,i)
+    - Result_NonHalt: the Turing machine does not halt
+    - Result_Unknown: the decider cannot conclude
+*)
+Fixpoint loop1_decider0(tm:TM Σ)(n:nat)(es:ListES)(d:Z)(ls:list (ListES*Z)):HaltDecideResult :=
 match n with
 | O => Result_Unknown
 | S n0 =>
@@ -20,16 +95,151 @@ match n with
     let ls' := ((es,d)::ls) in
     match n0 with
     | S n0' =>
-      loop1_decider0 tm n0 es' d' ls' n0' ns
+      loop1_decider0 tm n0 es' d' ls'
     | O =>
       if find_loop1_0 (es',d') (es,d) ls then Result_NonHalt else
-      loop1_decider0 tm n0 es' d' ls' (hd O ns) (tl ns)
+      loop1_decider0 tm n0 es' d' ls'
     end
   end
 end.
 
-Lemma loop1_decider0_def(tm:TM Σ)(n:nat)(es:ListES)(d:Z)(ls:list (ListES*Z))(n0:nat)(ns:list nat):
-loop1_decider0 tm n es d ls n0 ns =
+(** Loop decider
+
+Args:
+  - n: nat, gas parameter
+  - tm: TM Σ, the Turing machine that the NGramCPS decider is checking.
+
+Returns:
+  - HaltDecideResult:
+    - Result_Halt s i: the Turing machine halts at configuration (s,i)
+    - Result_NonHalt: the Turing machine does not halt
+    - Result_Unknown: the decider cannot conclude
+*)
+Definition loop1_decider(n:nat)(tm:TM Σ):HaltDecideResult :=
+  loop1_decider0 tm n {| l:=nil; r:=nil; m:=Σ0; s:=St0 |} Z0 nil.
+
+(* End: Loop decider implementation *)
+
+(* Begin: Proofs *)
+
+Lemma verify_loop1_spec tm h1 h2 ls1 ls2 n d:
+  (exists h0 ls0 n0 n1,
+  sidpos_history_WF tm h0 ls0 /\
+  (h1::ls1) = skipn n0 (h0::ls0) /\
+  (h2::ls2) = skipn (S n1) (h1::ls1) /\
+  sidpos_history_period h0 ls0 n0 (S n1) /\
+  n0+n=(S n1)) ->
+  verify_loop1 h1 h2 ls1 ls2 n d = true ->
+  ~ HaltsFromInit Σ Σ0 tm.
+Proof.
+  gd ls2. gd h2. gd h1. gd n.
+  induction ls1; intros.
+  - cbn in H0.
+    destruct h1,h2.
+    repeat rewrite andb_shortcut_spec in H0.
+    repeat rewrite Bool.andb_true_iff in H0.
+    repeat rewrite orb_shortcut_spec in H0.
+    repeat rewrite Bool.orb_true_iff in H0.
+    destruct H0 as [H0a [H0b [H0c _]]].
+    destruct H as [h0 [ls0 [N [T [Ha [Hb [Hc [Hd He]]]]]]]].
+    destruct n; cg.
+    cbn in Hc. rewrite skipn_nil in Hc. invst Hc.
+  - cbn in H0.
+    destruct h1,h2.
+    repeat rewrite andb_shortcut_spec in H0.
+    repeat rewrite Bool.andb_true_iff in H0.
+    repeat rewrite orb_shortcut_spec in H0.
+    repeat rewrite Bool.orb_true_iff in H0.
+    destruct H0 as [H0a [H0b H0c]].
+
+    destruct H as [h0 [ls0 [N [T [Ha [Hb [Hc [Hd He]]]]]]]].
+    St_eq_dec (s l) (s l0); cg.
+    Σ_eq_dec (m l) (m l0); cg.
+    clrs.
+
+    destruct ls2 as [|h2' ls2']; cg.
+    + destruct H0c as [H0c|H0c]; cg.
+      destruct n; cg.
+      epose proof (sidpos_history_period_S Hb Hc Hd H H0).
+      assert (N=S T) by lia; subst.
+      eapply loop1_nonhalt'; eauto 1.
+    + destruct H0c as [H0c|H0c].
+      * destruct n; cg.
+        epose proof (sidpos_history_period_S Hb Hc Hd H H0).
+        assert (N=S T) by lia; subst.
+        eapply loop1_nonhalt'; eauto 1.
+      * destruct n; cbn in H0c.
+        {
+          eapply IHls1; eauto 1.
+          destruct ls0 as [|h0' ls0'].
+          1: destruct N; [lia | cbn in Hb; rewrite skipn_nil in Hb; invst Hb].
+          exists h0'. exists ls0'. exists N. exists T.
+          repeat split; auto 1; try lia.
+          2,3: eapply skipn_S'; eauto 1.
+          1: eapply sidpos_history_WF_cdr,Ha.
+          destruct N as [|N]. 1: lia.
+          epose proof (sidpos_history_period_S' Hd) as Hd'. clear Hd.
+          cbn in Hb.
+          eapply sidpos_history_period_S; eauto 1.
+        }
+        {
+          eapply IHls1; eauto 1.
+          exists h0. exists ls0. exists (S N). exists T.
+          repeat split; auto 1; try lia.
+          1,2: eapply skipn_S; eauto 1.
+          apply (sidpos_history_period_S Hb Hc Hd H H0).
+        }
+Qed.
+
+
+
+Lemma find_loop1_spec tm h0 h1 h2 ls0 ls1 ls2 n:
+  sidpos_history_WF tm h0 ls0 ->
+  h1::ls1 = skipn (S n) (h0::ls0) ->
+  h2::ls2 = skipn (S n) (h1::ls1) ->
+  find_loop1 h0 h1 h2 ls0 ls1 ls2 n = true ->
+  ~ HaltsFromInit Σ Σ0 tm.
+Proof.
+  gd n. gd ls2. gd h2. gd h1.
+  induction ls1.
+  - intros. cbn in H2.
+    cbn in H1. rewrite skipn_nil in H1.
+    invst H1.
+  - intros. cbn in H2.
+    repeat rewrite orb_shortcut_spec in H2.
+    rewrite Bool.orb_true_iff in H2.
+    destruct H2 as [H2|H2].
+    + destruct h0 as [es0 d0].
+      destruct h1 as [es1 d1].
+      destruct h2 as [es2 d2].
+      repeat rewrite andb_shortcut_spec in H2.
+      repeat rewrite Bool.andb_true_iff in H2.
+      destruct H2 as [H2a [H2b [H2c [H2d H2e]]]].
+      eapply verify_loop1_spec; eauto 1.
+      eexists. eexists. exists 0. eexists.
+      repeat split; auto 1.
+      unfold sidpos_history_period. intros. lia.
+    + destruct ls2 as [|h3 [|h2' ls2']]; cg.
+      eapply IHls1; eauto 1.
+      * rewrite (skipn_S H0); cg.
+      * cbn in H1.
+        apply (skipn_S (skipn_S H1)).
+Qed.
+
+
+Lemma find_loop1_0_spec tm h0 h1 ls:
+  sidpos_history_WF tm h0 (h1::ls) ->
+  find_loop1_0 h0 h1 ls = true ->
+  ~HaltsFromInit Σ Σ0 tm.
+Proof.
+  intros.
+  unfold find_loop1_0 in H0.
+  destruct ls; cg.
+  eapply find_loop1_spec; eauto 1; reflexivity.
+Qed.
+
+Lemma loop1_decider0_def(tm:TM Σ)(n:nat)(es:ListES)(d:Z)(ls:list (ListES*Z)):
+loop1_decider0 tm n es d ls =
 match n with
 | O => Result_Unknown
 | S n0 =>
@@ -41,10 +251,10 @@ match n with
     let ls' := ((es,d)::ls) in
     match n0 with
     | S n0' =>
-      loop1_decider0 tm n0 es' d' ls' n0' ns
+      loop1_decider0 tm n0 es' d' ls' 
     | O =>
       if find_loop1_0 (es',d') (es,d) ls then Result_NonHalt else
-      loop1_decider0 tm n0 es' d' ls' (hd O ns) (tl ns)
+      loop1_decider0 tm n0 es' d' ls'
     end
   end
 end.
@@ -53,9 +263,9 @@ Proof.
   destruct n; cbn; reflexivity.
 Qed.
 
-Lemma loop1_decider0_spec tm n es d ls n0 ns:
+Lemma loop1_decider0_spec tm n es d ls:
   sidpos_history_WF tm (es,d) ls ->
-  match loop1_decider0 tm n es d ls n0 ns with
+  match loop1_decider0 tm n es d ls with
   | Result_Halt s0 i0 =>
     exists n1 es0,
     n1<n+(length ls) /\
@@ -66,7 +276,7 @@ Lemma loop1_decider0_spec tm n es d ls n0 ns:
   | Result_Unknown => True
   end.
 Proof.
-  gd ns. gd n0. gd ls. gd d. gd es.
+  gd ls. gd d. gd es.
   induction n; intros.
   1: cbn; trivial.
   destruct es as [l0 r0 m0 s0] eqn:Ees.
@@ -88,9 +298,9 @@ Proof.
       eapply find_loop1_0_spec; eauto 1.
       rewrite Heqt in Heqd'. cbn in Heqd'. subst d'. subst ls'. apply H0.
     + replace (let es'0 := es' in
-      let d'0 := d' in let ls'0 := ls' in loop1_decider0 tm (S n) es'0 d'0 ls'0 n ns) with
-      (loop1_decider0 tm (S n) es' d' ls' n ns) by reflexivity.
-      specialize (IHn _ _ _ n ns H0).
+      let d'0 := d' in let ls'0 := ls' in loop1_decider0 tm (S n) es'0 d'0 ls'0) with
+      (loop1_decider0 tm (S n) es' d' ls') by reflexivity.
+      specialize (IHn _ _ _ H0).
       rewrite Heqt in Heqd'. cbn in Heqd'. subst d'. subst ls'.
       replace (S n + length ((es, d) :: ls)) with (S (S n) + length ls) in IHn by (cbn; lia).
       apply IHn.
@@ -106,21 +316,18 @@ Proof.
     + subst es.  reflexivity.
 Qed.
 
-Definition loop1_decider(n:nat)(ns:list nat)(tm:TM Σ):HaltDecideResult :=
-  loop1_decider0 tm n {| l:=nil; r:=nil; m:=Σ0; s:=St0 |} Z0 nil (hd O ns) (tl ns).
-
-Lemma loop1_decider_WF BB n ns:
+Lemma loop1_decider_WF BB n:
   n<=S BB ->
-  HaltDecider_WF BB (loop1_decider n ns).
+  HaltDecider_WF BB (loop1_decider n).
 Proof.
   intros.
   unfold HaltDecider_WF,loop1_decider.
   intro tm.
   eassert (H0:_). {
-    apply (loop1_decider0_spec tm n {| l := nil; r := nil; m := Σ0; s := St0 |} 0 nil (hd 0 ns) (tl ns)).
+    apply (loop1_decider0_spec tm n {| l := nil; r := nil; m := Σ0; s := St0 |} 0 nil).
     apply sidpos_history_WF_O.
   }
-  destruct (loop1_decider0 tm n {| l := nil; r := nil; m := Σ0; s := St0 |} 0 nil (hd 0 ns) (tl ns)); auto 1.
+  destruct (loop1_decider0 tm n {| l := nil; r := nil; m := Σ0; s := St0 |} 0 nil); auto 1.
   cbn in H0.
   destruct H0 as [n1 [es0 [H0 [H1 [H2 [H3 H4]]]]]].
   destruct (ListES_toES es0) as [s1 t0] eqn:E0.
@@ -133,3 +340,5 @@ Proof.
   cbn in H3,H4. subst.
   apply H2.
 Qed.
+
+(* End: Proofs *)
